reachability

theories/Data/Graph.v
@@ -6,6 +6,7 @@ Require Import PnV.Prelude.X.
 
 #[local] Abbreviation In := L.In.
 #[local] Infix "\in" := E.In : type_scope.
+#[local] Infix "\subseteq" := E.isSubsetOf : type_scope.
 
 Universe U_vertices.
 
@@ -69,6 +70,11 @@ Variant Paths (v_s : V) (v_t : V) : ensemble (list V) :=
   | inPaths (p : list V)
     (H_path : v_s ---[ p ]--> v_t)
     : v_s :: p \in Paths v_s v_t.
+
+Variant Trails (v_s : V) (v_t : V) : ensemble (list V) :=
+  | inTrails (t : list V)
+    (H_path : v_s ===[ t ]==> v_t)
+    : v_s :: t \in Trails v_s v_t.
 
 Definition isAcyclic : Prop :=
   forall v : V, forall w : list V, v ~~~[ w ]~~> v -> w = [].
@@ -227,6 +233,201 @@ Proof.
 Defined.
 
 End deterministic_walk_to_sink_guarantees_sn.
+
+Section REACHABILITY.
+
+#[local] Notation "x ∈ xs" := (L.In x xs.(FSet.data)).
+
+Context {V_isPoset : isPoset V} {HsOrd_V : HsOrd V}.
+
+Variable nodes : fset V.
+
+Hypothesis arc_dec : forall v : V, forall v' : V, B.Decision ((v, v') \in E).
+
+Definition successors (v : V) : list V :=
+  filter (fun v' => decideb ((v, v') \in E)) nodes.(FSet.data).
+
+Lemma in_successors_iff (v : V) (v' : V)
+  : In v' (successors v) <-> v' ∈ nodes /\ (v, v') \in E.
+Proof.
+  unfold successors. rewrite filter_In. simpl; des_ifs; intuition congruence.
+Qed.
+
+Fixpoint reachables_worklist (fuel : nat) (seen : fset V) {struct fuel} : list V -> fset V :=
+  match fuel with
+  | O => fun _ => seen
+  | S fuel' =>
+    fix go (todo : list V) {struct todo} : fset V :=
+    match todo with
+    | [] => seen
+    | v :: todo' => if FS.mem v seen then go todo' else reachables_worklist fuel' (FS.add v seen) (successors v ++ todo')
+    end
+  end.
+
+Definition reachables (v : V) : fset V :=
+  reachables_worklist (length nodes.(FSet.data)) FS.empty [v].
+
+Lemma reachables_worklist_sound (P : V -> Prop) (fuel : nat) (seen : fset V) (todo : list V)
+  (CLOSED : forall v, forall v', P v -> (v, v') \in E -> P v')
+  (H_seen : forall v, v ∈ seen -> P v)
+  (H_todo : forall v, L.In v todo -> P v)
+  : forall v : V, forall IN : v ∈ reachables_worklist fuel seen todo, P v.
+Proof.
+  revert_until fuel. induction fuel as [ | fuel IH]; ii; auto.
+  revert_until todo. induction todo as [ | v todo IH_todo]; simpl; ii; auto. des_ifs.
+  - eapply IH_todo; auto.
+  - eapply IH with (seen := FS.add v seen) (todo := successors v ++ todo); auto.
+    + intros y H_y. rewrite FS.in_add_iff in H_y. des; ss; eauto.
+    + intros y H_y. rewrite in_app_iff in H_y. des; ss; auto.
+      eapply CLOSED with (v := v); ss; auto. now rewrite in_successors_iff in H_y.
+Qed.
+
+Hypothesis nodes_closed : forall v, v ∈ nodes -> forall v', (v, v') \in E -> v' ∈ nodes.
+
+Lemma walk_in_nodes (v : V) (v' : V) (w : list V)
+  (WALK : v ~~~[ w ]~~> v')
+  (IN : v ∈ nodes)
+  : v' ∈ nodes.
+Proof.
+  induction WALK; eauto.
+Qed.
+
+Lemma reachables_worklist_complete (fuel : nat) (seen : fset V) (todo : list V) (remaining : list V)
+  (H_seen : forall v, v ∈ seen -> v ∈ nodes)
+  (H_todo : forall v, L.In v todo -> v ∈ nodes)
+  (CLOSED : forall v, forall v', v ∈ seen -> (v, v') \in E -> (v' ∈ seen \/ In v' todo))
+  (COVER : forall v, v ∈ nodes -> (v ∈ seen \/ L.In v remaining))
+  (BOUND : length remaining <= fuel)
+  : forall v : V, forall v' : V, forall w : list V, forall FRONT : v ∈ seen \/ In v todo, forall H_walk : v ~~~[ w ]~~> v', v' ∈ reachables_worklist fuel seen todo.
+Proof.
+  revert_until fuel; induction fuel as [ | fuel IH]; simpl; i.
+  - assert (IN : v' ∈ nodes).
+    { eapply walk_in_nodes with (v := v) (w := w); auto. des; auto. }
+    obtain [YES | NO] with IN by COVER; auto.
+    destruct remaining; ss; lia.
+  - revert_until todo; induction todo as [ | v todo IH_todo]; simpl; i.
+    { des; [induction H_walk as [ | v0 v1 w EDGE WALK IH_walk] | tauto]; [auto | eapply IH_walk].
+      now find* [YES | []] by CLOSED.
+    }
+    { des_ifs.
+      - rewrite FS.mem_spec in Heq. eapply IH_todo with (remaining := remaining) (v := v0) (w := w); eauto.
+        + intros x y H_x H_edge. find* [YES | [EQ | YES]] by CLOSED; done.
+        + des; auto. left; congruence.
+      - rewrite FS.mem_spec in Heq.
+        assert (v_in_nodes : v ∈ nodes) by now eapply H_todo; left.
+        assert (v_in_remaining : L.In v remaining).
+        { find* [? | ?] by COVER; tauto. }
+        eapply IH with (remaining := remove (fun x => fun y => B.decide (x = y)) v remaining) (v := v0) (w := w); eauto.
+        + intros x x_in. rewrite FS.in_add_iff in x_in. destruct x_in; eauto.
+        + intros x x_in. rewrite L.in_app_iff in x_in. destruct x_in as [x_in | x_in].
+          * now rewrite in_successors_iff in x_in.
+          * eapply H_todo. now right.
+        + intros x y x_in H_edge. rewrite FS.in_add_iff in x_in. destruct x_in as [EQ | IN].
+          * subst x. right. rewrite in_app_iff. left. rewrite in_successors_iff; eauto.
+          * rewrite FS.in_add_iff. rewrite L.in_app_iff.
+            find* [YES | [EQ | YES]] by CLOSED; tauto.
+        + intros x x_in. destruct (FS.mem x (FS.add v seen)) eqn: H_OBS.
+          * left. now rewrite FS.mem_spec in H_OBS.
+          * right. rewrite FS.mem_spec in H_OBS. rewrite FS.in_add_iff in H_OBS. rewrite L.in_remove_iff.
+            find* ? by COVER; split; intuition congruence.
+        + obtain ? with v_in_remaining by (remove_length_lt (EQ_DEC := fun x => fun y => B.decide (x = y))).
+          lia.
+        + rewrite FS.in_add_iff. rewrite L.in_app_iff. done.
+    }
+Qed.
+
+Theorem reachables_correct (v : V)
+  (IN : v ∈ nodes)
+  : forall v' : V, v' ∈ reachables v <-> (exists w, w \in Walks v v').
+Proof.
+  split.
+  - intros REACHABLE. unfold reachables in REACHABLE.
+    enough (exists w, v ~~~[ w ]~~> v') as [w H_walk] by now exists (v :: w); econs.
+    eapply reachables_worklist_sound with (P := fun x => exists w, v ~~~[ w ]~~> x) (fuel := length nodes.(FSet.data)) (seen := FS.empty) (todo := [v]).
+    + intros x y [w WALK] EDGE. exists (w ++ [y]). eapply walk_app; eauto.
+    + intros x. rewrite FS.in_empty_iff. tauto.
+    + simpl. intros x [EQ | []]. subst x. exists []. econs 1.
+    + exact REACHABLE.
+  - intros [w WALK]. inversion WALK as [w' H_walk]; subst; clear WALK.
+    eapply reachables_worklist_complete with (remaining := nodes.(FSet.data)) (v := v) (w := w'); simpl; done.
+Qed.
+
+End REACHABILITY.
+
+Section PROPAGATION.
+
+#[local] Notation "x ∈ xs" := (L.In x xs.(FSet.data)).
+
+Context {X : Type} {V_isPoset : isPoset V} {X_isPoset : isPoset X} {HsOrd_V : HsOrd V} {HsOrd_X : HsOrd X}.
+
+Variable seed : fpmap V (fset X).
+
+Definition lookup_seed (v : V) : fset X :=
+  match FPM.lookup v seed with
+  | None => FS.empty
+  | Some xs => xs
+  end.
+
+Inductive propagate_trace (v : V) (x : X) : ensemble (list V) :=
+  | propagate_trace_init
+    (H_in_seed : x ∈ lookup_seed v)
+    : [] \in propagate_trace v x
+  | propagate_trace_step (v' : V) (w : list V)
+    (H_edge : (v, v') \in E)
+    (H_in_closure : w \in propagate_trace v' x)
+    : v' :: w \in propagate_trace v x.
+
+#[local] Hint Constructors propagate_trace : core.
+
+Lemma propagate_trace_iff (v : V) (x : X) (w : list V)
+  : w \in propagate_trace v x <-> (exists v', v ~~~[ w ]~~> v' /\ x ∈ lookup_seed v').
+Proof.
+  split.
+  - intros H_trace. induction H_trace; des; eauto.
+  - intros (v' & H_walk & H_in_seed). induction H_walk; eauto.
+Qed.
+
+Variable nodes : fset V.
+
+Definition recursive_equation (F : V -> ensemble X) : Prop :=
+  forall v : V, forall IN : v ∈ nodes, forall x : X, x \in F v <-> ⟪ UNFOLD : x ∈ lookup_seed v \/ (exists v', x \in F v' /\ (v, v') \in E) ⟫.
+
+Hypothesis arc_dec : forall v : V, forall v' : V, B.Decision ((v, v') \in E).
+
+Definition least_solution (v : V) : fset X :=
+  FS.bind (reachables nodes arc_dec v) lookup_seed.
+
+Hypothesis nodes_closed : forall v, v ∈ nodes -> forall v', (v, v') \in E -> v' ∈ nodes.
+
+Theorem least_solution_correct (v : V)
+  (IN : v ∈ nodes)
+  : forall x : X, x ∈ least_solution v <-> (exists w, w \in propagate_trace v x).
+Proof.
+  intros x. unfold least_solution. rewrite FS.in_bind_iff. split.
+  - intros (v' & H_reachable & H_in_seed).
+    rewrite reachables_correct in H_reachable by eauto.
+    destruct H_reachable as [w H_walks]. inv H_walks.
+    eexists. rewrite propagate_trace_iff. eauto.
+  - intros [w H_trace]. rewrite propagate_trace_iff in H_trace.
+    destruct H_trace as (v' & H_walk & H_in_seed). exists v'. split; auto.
+    rewrite reachables_correct by eauto. exists (v :: w). econs; eauto.
+Qed.
+
+Theorem least_solution_of_recursive_equation
+  : recursive_equation (fun v : V => { x : X | x ∈ least_solution v }%function) /\ ⟪ LEAST : forall F, recursive_equation F -> forall v, v ∈ nodes -> E.fromList (least_solution v).(FSet.data) \subseteq F v ⟫.
+Proof.
+  split.
+  - intros v IN x. unnw. unfold E.In at 1 2. rewrite least_solution_correct by eauto. split.
+    + intros [w H_trace]. inv H_trace; auto. right. esplits; eauto. rewrite least_solution_correct; eauto.
+    + intros [H_in_seed | (v' & H_in_solution & H_edge)]; eauto.
+      rewrite least_solution_correct in H_in_solution by eauto.
+      destruct H_in_solution as [w H_trace]. exists (v' :: w). econs; eauto.
+  - intros F H_rec v IN x H_x. rewrite E.in_fromList_iff in H_x.
+    rewrite least_solution_correct in H_x by eauto.
+    destruct H_x as [w H_trace]. induction H_trace; eapply H_rec; eauto. right; esplits; eauto.
+Qed.
+
+End PROPAGATION.
 
 End Digraph.
 
